Also implement Assert

src/goose_lang/lib/control/impl.v
@@ -7,4 +7,8 @@ Definition Assume: val :=
   λ: "cond", if: Var "cond" then #()
              else (rec: "loop" <> := Var "loop" #()) #().
 
+Definition Assert: val :=
+  λ: "cond", if: Var "cond" then #()
+             else Panic "assert failed".
+
 End goose_lang.
